Scalar universality a and c

SemanticsTesting/02ScalarsUniversal.lean
@@ -3,13 +3,40 @@ import SemanticsTesting.«02Scalars»
 
 open SpLean.Algebraic
 
--- Every phase e^{iθ} is realised by a scalar diagram: √2 e^{iθ} · 1/√2
-lemma scalar_univ_euler_form (θ : Phase) :
-    ∃ d : ZX 0 0, ∀ f g : Wires 0, d.sem f g = Complex.exp (θ.angle * Complex.I) := by
-  use redPiCircleAnyGreen θ ≫ redCircleTripleLinkGreenCircle
-  intro f g
+-- pqs ex 3.5
+-- By combining the diagrams from 02Scalars,
+--   find a ZX-diagram to represent the following scalar values z:
+
+-- a) z = -1
+abbrev scalarDiagNegOne := redPiCircleAnyGreen ⟨1, 1⟩ ≫ redCircleTripleLinkGreenCircle
+#zx scalarDiagNegOne
+lemma scalar_univ_neg_one (f g : Wires 0) :
+  scalarDiagNegOne.sem f g = -1 := by
+  rw [ZX.sem, Finset.univ_unique, Finset.sum_singleton]
+  rw [scalar_sem_sqrt_two_e_i_alpha, scalar_sem_one_over_sqrt_two, Phase.angle]
+  unfold rootTwo eiTheta
+  norm_num
+
+
+-- b) z = e^{i θ} for any θ
+abbrev scalarDiagEuler (θ : Phase) := redPiCircleAnyGreen θ ≫ redCircleTripleLinkGreenCircle
+#zx scalarDiagEuler ⟨1, 4⟩
+lemma scalar_univ_euler_form (θ : Phase) (f g : Wires 0) :
+    (scalarDiagEuler θ).sem f g = eiTheta θ.angle := by
   -- Composition of scalars is a sum over the unique element of `Wires 0`
   rw [ZX.sem, Finset.univ_unique, Finset.sum_singleton,
     scalar_sem_sqrt_two_e_i_alpha, scalar_sem_one_over_sqrt_two]
   unfold rootTwo eiTheta
   field_simp
+
+-- c) z = 1/2
+abbrev scalarDiagHalf := redCircleTripleLinkGreenCircle ≫ redCircleTripleLinkGreenCircle
+#zx scalarDiagHalf
+lemma scalar_univ_half (f g : Wires 0) :
+  scalarDiagHalf.sem f g = 1/2 := by
+  rw [ZX.sem, Finset.univ_unique, Finset.sum_singleton]
+  rw [scalar_sem_one_over_sqrt_two, scalar_sem_one_over_sqrt_two]
+  unfold rootTwo
+  norm_cast
+  ring_nf
+  norm_num
